Deletion on interval trees.

HOL/DataStrs/BST_Func.thy
@@ -35,40 +35,31 @@ section {* Deletion on trees *}
 
 fun del_min :: "('a, 'b) tree \<Rightarrow> ('a \<times> 'b) \<times> ('a, 'b) tree" where
   "del_min Tip = undefined"
-| "del_min (Node Tip x v rt) = ((x, v), rt)"
-| "del_min (Node lt x v rt) = (fst (del_min lt), Node (snd (del_min lt)) x v rt)"
-setup {* fold add_rewrite_rule @{thms del_min.simps(2-3)} *}
+| "del_min (Node lt x v rt) =
+   (if lt = Tip then ((x, v), rt) else
+    (fst (del_min lt), Node (snd (del_min lt)) x v rt))"
+setup {* add_rewrite_rule @{thm del_min.simps(2)} *}
 
-theorem delete_min_del_hd [rewrite]:
+lemma delete_min_del_hd [rewrite]:
   "t \<noteq> Tip \<Longrightarrow> fst (fst (del_min t)) # in_traverse (snd (del_min t)) = in_traverse t"
-@proof
-  @induct t @with
-    @subgoal "t = Node l x v r" @case "l = Tip" @endgoal
-  @end
-@qed
+@proof @induct t @qed
 
-theorem delete_min_del_hd_pairs [rewrite]:
+lemma delete_min_del_hd_pairs [rewrite]:
   "t \<noteq> Tip \<Longrightarrow> fst (del_min t) # in_traverse_pairs (snd (del_min t)) = in_traverse_pairs t"
-@proof
-  @induct t @with
-    @subgoal "t = Node l x v r" @case "l = Tip" @endgoal
-  @end
-@qed
+@proof @induct t @qed
 
 fun delete_elt_tree :: "('a, 'b) tree \<Rightarrow> ('a, 'b) tree" where
   "delete_elt_tree Tip = undefined"
-| "delete_elt_tree (Node Tip x v rt) = rt"
-| "delete_elt_tree (Node lt x v Tip) = lt"
-| "delete_elt_tree (Node lt x v rt) = Node lt (fst (fst (del_min rt))) (snd (fst (del_min rt))) (snd (del_min rt))"
-setup {* fold add_rewrite_rule @{thms delete_elt_tree.simps(2-4)} *}
+| "delete_elt_tree (Node lt x v rt) =
+    (if lt = Tip then rt else if rt = Tip then lt else
+     Node lt (fst (fst (del_min rt))) (snd (fst (del_min rt))) (snd (del_min rt)))"
+setup {* add_rewrite_rule @{thm delete_elt_tree.simps(2)} *}
 
-theorem delete_elt_in_traverse [rewrite]:
-  "in_traverse (delete_elt_tree (Node lt x v rt)) = in_traverse lt @ in_traverse rt"
-@proof @case "lt = Tip" @then @case "rt = Tip" @qed
+lemma delete_elt_in_traverse [rewrite]:
+  "in_traverse (delete_elt_tree (Node lt x v rt)) = in_traverse lt @ in_traverse rt" by auto2
 
-theorem delete_elt_in_traverse_pairs [rewrite]:
-  "in_traverse_pairs (delete_elt_tree (Node lt x v rt)) = in_traverse_pairs lt @ in_traverse_pairs rt"
-@proof @case "lt = Tip" @then @case "rt = Tip" @qed
+lemma delete_elt_in_traverse_pairs [rewrite]:
+  "in_traverse_pairs (delete_elt_tree (Node lt x v rt)) = in_traverse_pairs lt @ in_traverse_pairs rt" by auto2
 
 fun tree_delete :: "'a::ord \<Rightarrow> ('a, 'b) tree \<Rightarrow> ('a, 'b) tree" where
   "tree_delete x Tip = Tip"
@@ -78,18 +69,18 @@ fun tree_delete :: "'a::ord \<Rightarrow> ('a, 'b) tree \<Rightarrow> ('a, 'b) t
      else Node l y w (tree_delete x r))"
 setup {* fold add_rewrite_rule @{thms tree_delete.simps} *}
 
-theorem tree_delete_in_traverse [rewrite]:
+lemma tree_delete_in_traverse [rewrite]:
   "tree_sorted t \<Longrightarrow> in_traverse (tree_delete x t) = remove_elt_list x (in_traverse t)"
 @proof @induct t @qed
 
-theorem tree_delete_in_traverse_pairs [rewrite]:
+lemma tree_delete_in_traverse_pairs [rewrite]:
   "tree_sorted t \<Longrightarrow> in_traverse_pairs (tree_delete x t) = remove_elt_pairs x (in_traverse_pairs t)"
 @proof @induct t @qed
 
-theorem tree_delete_sorted [forward]:
+lemma tree_delete_sorted [forward]:
   "tree_sorted t \<Longrightarrow> tree_sorted (tree_delete x t)" by auto2
 
-theorem tree_delete_map [rewrite]:
+lemma tree_delete_map [rewrite]:
   "tree_sorted t \<Longrightarrow> tree_map (tree_delete x t) = delete_map x (tree_map t)" by auto2
 
 section {* Search on sorted trees *}
